Abstracted LM_EM over language so it can be used in fuel_termination without specializing to heap_lang

fairness/heap_lang/em_lm.v
@@ -1,42 +1,50 @@
 From trillium.fairness Require Export fairness resources fair_termination fuel fuel_ext. 
-From trillium.fairness.heap_lang Require Export lang heap_lang_defs.
+(* From trillium.fairness.heap_lang Require Export lang heap_lang_defs. *)
 From iris.proofmode Require Import tactics.
 From trillium.fairness Require Export partial_ownership.
+From trillium.fairness Require Import execution_model.
 
+Section LMExecModel.
+  Context `{LM:LiveModel (locale Λ) M}.
+  Context `{CNT_Λ: Countable (locale Λ)}. 
 
-Definition LM_init_resource `{LM:LiveModel (locale heap_lang) M} `{!fairnessGS LM Σ}
+  (* TODO: remove *)
+  Context (τ0: locale Λ). 
+  Hypothesis (INITτ0: forall e, locales_of_list [e] = [τ0]). 
+
+Definition LM_init_resource `{!fairnessGS LM Σ}
    (s1: LM)
   (* FR *)
   : iProp Σ :=
   frag_model_is s1 ∗
   (∃ FR, frag_free_roles_are (FR ∖ live_roles _ s1)) ∗
-  has_fuels (Σ := Σ) 0%nat (gset_to_gmap (LM.(lm_fl) s1) (M.(live_roles) s1))
+  has_fuels (Σ := Σ) τ0 (gset_to_gmap (LM.(lm_fl) s1) (M.(live_roles) s1))
   (PMPP := ActualOwnershipPartialPre). 
 
-Definition init_thread_post `{LM:LiveModel (locale heap_lang) M} `{!fairnessGS LM Σ}
-  (tid: locale heap_lang): iProp Σ :=
+Definition init_thread_post `{!fairnessGS LM Σ}
+  (tid: locale Λ): iProp Σ :=
   (* tid ↦M ∅. *)
   frag_mapping_is {[ tid := ∅ ]}.
 
-Definition lm_model_init `{LM: LiveModel (locale heap_lang) M} (δ: mstate LM) :=
+Definition lm_model_init (δ: mstate LM) :=
   ls_fuel δ = gset_to_gmap (lm_fl LM δ) (live_roles _ (ls_under δ)) /\
   (* ls_mapping δ = gset_to_gmap 0%nat (live_roles _ (ls_under δ)).  *)
-  ls_tmap δ (LM := LM) = {[ 0%nat := live_roles _ (ls_under δ) ]}. 
+  ls_tmap δ (LM := LM) = {[ τ0 := live_roles _ (ls_under δ) ]}. 
 
-Definition lm_cfg_init (σ: cfg heap_lang) :=
-  exists (e: expr), σ.1 = [e].
+Definition lm_cfg_init (σ: cfg Λ) :=
+  exists (e: expr Λ), σ.1 = [e].
 
-Definition lm_is_init_st `{LM: LiveModel (locale heap_lang) M} σ s := 
-  lm_cfg_init σ /\ lm_model_init s (LM := LM). 
+Definition lm_is_init_st σ s := 
+  lm_cfg_init σ /\ lm_model_init s. 
 
 Definition tids_restrict `{M: FairModel} `{Countable (locale Λ)}
   (c: cfg Λ) (tmap: gmap (locale Λ) (gset (fmrole M))): Prop :=
   forall ζ, ζ ∉ locales_of_list c.1 → tmap !! ζ = None.
 
 (* TODO: unify with existing locales_of_list_from_locale_from, 
-   remove restriction for heap_lang *)
+   remove restriction for Λ *)
 Lemma locales_of_list_from_locale_from' tp0 tp1 ζ:
-  ζ ∈ locales_of_list_from tp0 tp1 (Λ := heap_lang) ->
+  ζ ∈ locales_of_list_from tp0 tp1 (Λ := Λ) ->
   is_Some (from_locale_from tp0 tp1 ζ).
 Proof.
   clear -tp0 tp1 ζ.
@@ -49,7 +57,7 @@ Proof.
   set_solver.
 Qed.
 
-Lemma tids_restrict_smaller `{LM:LiveModel (locale heap_lang) M} (σ: cfg heap_lang) (δ: lm_ls LM):
+Lemma tids_restrict_smaller (σ: cfg Λ) (δ: lm_ls LM):
   tids_restrict σ (ls_tmap δ) -> tids_smaller σ.1 δ.
 Proof.
   rewrite /tids_smaller /tids_restrict. 
@@ -60,17 +68,18 @@ Proof.
   congruence. 
 Qed. 
 
-Definition em_lm_msi `{LM:LiveModel (locale heap_lang) M} `{!fairnessGS LM Σ}
-  (c: cfg heap_lang) (δ: mstate LM): iProp Σ :=
+Definition em_lm_msi `{!fairnessGS LM Σ}
+  (c: cfg Λ) (δ: mstate LM): iProp Σ :=
   model_state_interp δ ∗ ⌜ tids_restrict c (ls_tmap δ (LM := LM)) ⌝. 
 
 (* TODO: how to make 'heap..' instantiations less wordy? *)
 (* TODO: how to avoid different instances of EqDec and Cnt? *)
-Lemma init_fairnessGS_LM Σ `{hPre: @fairnessGpreS (locale heap_lang) M LM Σ
-                                     Nat.eq_dec nat_countable
-  }
-  (* `(LM:LiveModel heap_lang M)   *)
-  (s1: LM) (σ1 : cfg heap_lang) (INIT: lm_is_init_st σ1 s1):
+Lemma init_fairnessGS_LM Σ
+  (* `{hPre: @fairnessGpreS (locale Λ) M LM Σ Nat.eq_dec nat_countable} *)
+  `{hPre: @fairnessGpreS (locale Λ) M LM Σ _ CNT_Λ}
+
+  (* `(LM:LiveModel Λ M)   *)
+  (s1: LM) (σ1 : cfg Λ) (INIT: lm_is_init_st σ1 s1):
   ⊢ (|==> ∃ fGS: fairnessGS LM Σ, (* TODO: what is a canonical way of doing it? *)
        (* ∀ `{hGS: @heapGS Σ _ (@LM_EM _ LM)}, *)
        (*   ⌜ hGS.(heap_fairnessGS) = fGS⌝ → *)
@@ -113,7 +122,9 @@ Proof.
   iSplitL.
   2: { iPureIntro. rewrite /tids_restrict.
        intros tid Hlocs. rewrite TMAP lookup_singleton_ne //.
-       compute in Hlocs. set_solver. }
+       (* compute in Hlocs. *)
+       simpl in Hlocs. rewrite INITτ0 in Hlocs. 
+       set_solver. }
 
   rewrite /LM_init_resource /has_fuels /=.
   rewrite dom_gset_to_gmap. rewrite FUEL TMAP. iFrame.
@@ -135,16 +146,16 @@ Proof.
 Qed.
 
 
-Global Instance LM_EM `{LM: LiveModel (locale heap_lang) M}: @ExecutionModel heap_lang LM.
+Global Instance LM_EM: @ExecutionModel Λ LM.
 refine
   {|
     em_preGS := fun Σ => fairnessGpreS LM Σ;
     em_GS := fun Σ => fairnessGS LM Σ;
-    em_Σ := fairnessΣ (locale heap_lang) M;
+    em_Σ := fairnessΣ (locale Λ) M;
     em_Σ_subG := fun Σ => @subG_fairnessGpreS _ _ _ LM _ _;
 
     (* em_valid_evolution_step := valid_evolution_step (LM := LM); *)
-    em_thread_post Σ := fun {_: fairnessGS LM Σ} (tid: locale heap_lang) => 
+    em_thread_post Σ := fun {_: fairnessGS LM Σ} (tid: locale Λ) => 
                           (* tid ↦M ∅; *)
                           frag_mapping_is {[ tid := ∅ ]};
     (* TODO: cannot express the msi instantiation this way*)
@@ -156,272 +167,10 @@ refine
 (* TODO: cannot directly specify these components *)
 Unshelve. 
 { exact (valid_evolution_step (LM := LM)). }
-2: { intros ? fG. exact (em_lm_msi (LM := LM) (fairnessGS0 := fG)). } 
+2: { intros ? fG. exact (em_lm_msi (fairnessGS0 := fG)). } 
 intros. iIntros. iMod (init_fairnessGS_LM _ s1 σ) as "[% [? X]]"; [done| ]. 
 iModIntro. iExists _. iFrame. 
 Defined. 
 
-(* TODO: get rid of it*)
-Global Instance LM_EM_fairPre `{LM: LiveModel (locale heap_lang) M}
-                `{hGS: @heapGpreS Σ LM (@LM_EM _ LM)}:
-  fairnessGpreS LM Σ.
-Proof. apply hGS. Defined. 
+End LMExecModel.
 
-(* TODO: get rid of it*)
-Global Instance LM_EM_fair `{LM: LiveModel (locale heap_lang) M}
-                `{hGS: @heapGS Σ LM (@LM_EM _ LM)}:
-  fairnessGS LM Σ.
-Proof. apply hGS. Defined.
-
-Lemma tids_smaller_restrict_mapping `{M: FairModel}
-
-  (c1 c2: cfg heap_lang) δ1 δ2 (ζ: locale heap_lang)
-  (Hζs : tids_smaller c1.1 δ1)
-  (DOM12: ls_mapping δ2 ⊆ ls_mapping δ1)
-  (STEP: locale_step c1 (Some ζ) c2)
-  :
-  tids_smaller c2.1 δ2 (M := M).
-Proof.
-  unfold tids_smaller; simpl.
-  intros ρ ζ0 Hin.
-  destruct c1, c2.
-  eapply from_locale_step =>//.
-  rewrite /tids_smaller /= in Hζs. eapply Hζs.
-  eapply lookup_weaken; eauto. 
-Qed.
-
-Lemma tids_dom_restrict_mapping `{LM: LiveModel (locale heap_lang) M} 
-  (c1 c2: cfg heap_lang)
-  (tmap1 tmap2: gmap (locale heap_lang) (gset (fmrole M))) (ζ: locale heap_lang)
-  (Hstep : locale_step c1 (Some ζ) c2)
-  (Hlocssmall: tids_restrict c1 tmap1)
-  (TMAP2: exists S, tmap2 = <[ζ:=S]> (tmap1))
-  :
-  tids_restrict c2 tmap2.
-Proof.
-  intros ζ0 Hnotin.
-  destruct TMAP2 as [? ->]. 
-  destruct c1, c2. simpl in *. 
-  apply lookup_insert_None; split.
-  + apply Hlocssmall.
-    have Hle := locales_of_list_step_incl _ _ _ _ _ Hstep. simpl.
-    clear -Hnotin Hle. set_solver.
-  + intros <-. 
-    have ? := locales_of_list_step_incl _ _ _ _ _ Hstep. simpl.
-    (* clear Hfueldom Hsamedoms. *)
-    inversion Hstep. simplify_eq.
-    assert (locale_of t1 e1 ∈ locales_of_list (t1 ++ e1 :: t2));
-      last by eauto.
-    apply locales_of_list_from_locale_from.
-    rewrite from_locale_from_Some //. 
-    eapply prefixes_from_spec.
-    eexists _,_. by list_simplifier.
-Qed.
-  (* TODO: ?? *)
-    (* - rewrite Hnewdom /new_dom. apply elem_of_equiv_empty_L. intros ρ [Hin1 Hin2]%elem_of_intersection. *)
-    (*   assert (ρ ∈ dom (ls_fuel δ1)) *)
-    (*     by set_solver -Hnewdom Hsamedoms Hfueldom. *)
-    (*   set_solver -Hnewdom Hsamedoms Hfueldom. } *) 
-
-
-Lemma tids_smaller_fork_step `{LM: LiveModel (locale heap_lang) M}  σ1 σ2 δ1 δ2 ζ τ_new
-  (Hstep: locale_step σ1 (Some ζ) σ2)
-  (SM: tids_smaller σ1.1 δ1)
-  (MAP2: exists (R2: gset (fmrole M)), ls_mapping δ2 = map_imap
-                                                    (λ (ρ : fmrole M) (o : locale heap_lang),
-                                                      if decide (ρ ∈ R2) then Some τ_new else Some o)
-                                                    (ls_mapping δ1))
-  (FORK: ∃ tp1' efork, τ_new = locale_of σ1.1 efork /\ σ2.1 = tp1' ++ [efork] ∧ length tp1' = length σ1.1)
-  :
-  tids_smaller σ2.1 δ2 (M := M).
-Proof.
-  destruct σ1 as [tp1 σ1], σ2 as [tp2 σ2]. simpl in *.
-  intros ρ ζ'.
-  simpl in *. destruct MAP2 as [R2 ->].
-  simpl. rewrite map_lookup_imap.
-  destruct (ls_mapping δ1 !!ρ) eqn:Heq.
-  2: { intros. simpl in *. discriminate. }
-  
-  destruct (decide (ρ ∈ R2)); first  (intros ?; simplify_eq).
-  - destruct FORK as (tp1' & efork & (-> & -> & Hlen)).
-    inversion Hstep as [? ? e1 ? e2 ? efs t1 t2 Hf1 YY Hprimstep |]. simplify_eq.
-    assert (efs = [efork]) as ->.
-    { symmetry. assert (length tp1' = length (t1 ++ e2 :: t2)).
-      rewrite app_length //=; rewrite app_length //= in Hlen.
-      clear Hlen. eapply app_inj_1 =>//. by list_simplifier. }
-    inversion H.
-    subst ζ'. 
-    assert (is_Some (from_locale (t1 ++ e1 :: t2 ++ [efork]) (locale_of (t1 ++ e1 :: t2) efork))).
-    + unfold from_locale. erewrite from_locale_from_Some; eauto.
-      apply prefixes_from_spec. list_simplifier. eexists _, []. split=>//.
-      by list_simplifier.
-    + eapply from_locale_from_equiv =>//; [constructor |].
-      (* rewrite H0. *)
-      replace (t1 ++ e1 :: t2 ++ [efork]) with ((t1 ++ e1 :: t2) ++ [efork]);
-        last by list_simplifier.
-      replace (t1 ++ e2 :: t2 ++ [efork]) with ((t1 ++ e2 :: t2) ++ [efork]);
-        last by list_simplifier.
-      assert (locales_equiv (t1 ++ e1 :: t2) (t1 ++ e2 :: t2)).
-      { apply locales_equiv_middle. eapply locale_step_preserve =>//. }
-      assert (tp1' = t1 ++ e2 :: t2).
-      { rewrite app_comm_cons in YY. 
-        erewrite app_assoc in YY. eapply app_inj_tail in YY. apply YY. }
-      apply locales_equiv_from_app =>//.
-      * congruence.
-      * eapply locales_equiv_from_refl. by list_simplifier. 
-  - intros ?; simplify_eq.
-    assert (is_Some (from_locale tp1 ζ')). 
-    2: by eapply from_locale_step =>//.
-    inversion H. subst. eauto. 
-Qed.
-
-Lemma tids_dom_fork_step `{LM: LiveModel (locale heap_lang) M}
-  (c1 c2: cfg heap_lang) (ζ: locale heap_lang)
-  (tmap1 tmap2: gmap (locale heap_lang) (gset (fmrole M)))
-  τ_new (R1 R2: gset (fmrole M))
-  (Hstep: locale_step c1 (Some ζ) c2)
-  (Hsmall: ∀ ζ : locale heap_lang,
-      ζ ∉ locales_of_list c1.1 → tmap1 !! ζ = None)
-  (Hmapping : ζ ∈ dom tmap1)
-  (FORK: (∃ tp1' efork, τ_new = locale_of c1.1 efork /\ c2.1 = tp1' ++ [efork] ∧ length tp1' = length c1.1))
-  (TMAP2: tmap2 = <[τ_new:=R2]> (<[ζ:=R1]> (tmap1)))
-  :
-  ∀ ζ0 : locale heap_lang,
-    ζ0 ∉ locales_of_list c2.1 → tmap2 !! ζ0 = None.
-Proof.
-  assert (Hlocincl: locales_of_list c1.1 ⊆ locales_of_list c2.1).
-  { destruct c1 as [tp1 σ1], c2 as [tp2 σ2]. simpl in *.
-    apply (locales_of_list_step_incl _ _ _ _ _ Hstep). }
-  intros ζ' Hζ'.
-  rewrite TMAP2.
-  destruct c1 as [tp1 σ1], c2 as [tp2 σ2]. simpl in *.
-  rewrite lookup_insert_ne.
-  { rewrite lookup_insert_ne; last first.
-    { intros <-.
-      apply elem_of_dom in Hmapping as [? MM]. 
-      rewrite Hsmall in MM; [congruence | naive_solver]. }
-    apply Hsmall; set_unfold; naive_solver. }
-  pose proof (locales_of_list_step_incl _ _ _ _ _ Hstep).
-  (* clear Hfueldom Hsamedoms. *)
-  assert (ζ' ∉ locales_of_list tp1) by eauto.
-  intros contra. simplify_eq.
-  destruct FORK as (tp1' & efork & (-> & -> & Hlen)).
-  inversion Hstep as [? ? e1 ? e2 ? efs t1 t2 Hf1 YY Hprimstep |].
-  simplify_eq.
-  assert (efs = [efork]) as ->.
-  { symmetry. assert (length tp1' = length (t1 ++ e2 :: t2)).
-    rewrite app_length //=; rewrite app_length //= in Hlen.
-    clear Hlen. eapply app_inj_1 =>//. by list_simplifier. }
-  (* rewrite H0 in Hζ'. *)
-  apply Hζ'. apply elem_of_list_fmap.
-  eexists (t1 ++ e2 :: t2, _); split =>//.
-  - erewrite locale_equiv =>//. apply locales_equiv_middle.
-    eapply locale_step_preserve => //.
-  - replace (t1 ++ e2 :: t2 ++ [efork]) with ((t1 ++ e2 :: t2) ++ [efork]); last by list_simplifier.
-    rewrite prefixes_from_app.
-    rewrite app_comm_cons app_assoc in YY. eapply app_inj_tail in YY.
-    set_unfold; naive_solver.
-Qed.
-
-
-Lemma tids_smaller_model_step `{LM: LiveModel (locale heap_lang) M} c1 c2 ζ δ1 δ2
-  (Hstep: locale_step c1 (Some ζ) c2)
-  (Hless: tids_smaller c1.1 δ1)
-  (* S is a subset of dom (ls_fuel δ1); *)
-  (*      missing roles are those that are dropped by ζ; *)
-  (*      new roles get assigned here *)
-  (MAP2: exists f (S: gset (fmrole M)),
-      ls_mapping δ2 = map_imap
-                        (λ (ρ' : fmrole M) (_ : nat),
-                          if decide (ρ' ∈ dom (ls_fuel δ1))
-                          then ls_mapping δ1 !! ρ'
-                          else Some ζ)
-                        (gset_to_gmap f S)
-  )
-  :
-  tids_smaller c2.1 δ2 (M := M).
-Proof.  
-  (* eapply tids_smaller_restrict_mapping; eauto. *)
-  (* destruct MAP2 as (?&?&->).   *)
-  unfold tids_smaller; simpl.
-  simpl in MAP2. destruct MAP2 as (?&S&->).
-  intros ρ' ? Hmim.
-  rewrite map_lookup_imap in Hmim. rewrite lookup_gset_to_gmap in Hmim.
-  destruct (decide (ρ' ∈ S)); last by rewrite option_guard_False in Hmim.
-  rewrite option_guard_True //= in Hmim.
-  destruct (decide (ρ' ∈ dom (ls_fuel δ1))). 
-  + inversion Hstep; simplify_eq.
-    eapply from_locale_step =>//. eapply Hless. rewrite -Hmim decide_True; auto. 
-  + simplify_eq.
-    inversion Hstep; simplify_eq.
-    eapply from_locale_step =>//. unfold from_locale.
-    simpl. rewrite decide_False in Hmim; [| done]. inversion Hmim. subst ζ0.  
-    rewrite from_locale_from_Some; [done| ]. 
-    apply prefixes_from_spec. exists t1, t2. by list_simplifier.
-Qed.
-
-Ltac by_contradiction :=
-  match goal with
-  | |- ?goal => destruct_decide (decide (goal)); first done; exfalso
-  end.
-
-Lemma mim_helper_model_step `{LM: LiveModel (locale heap_lang) M}
-  (s2 : M)
-  (fs1 fs2 : gmap (fmrole M) nat)
-  (ρ : fmrole M)
-  (δ1 : LM)
-  (ζ : locale heap_lang)
-  (fr1 : gset (fmrole M))
-  (Hfr_new : live_roles M s2 ∖ live_roles M δ1 ⊆ fr1)
-  (Hfuelsval : valid_new_fuelmap fs1 fs2 δ1 s2 ρ (LM := LM))
-  (Hxdom : ∀ ρ : fmrole M, ls_mapping δ1 !! ρ = Some ζ ↔ ρ ∈ dom fs1)
-  (HFR : fr1 ∩ dom (ls_fuel δ1) = ∅):
-  maps_inverse_match
-    (map_imap
-       (λ (ρ' : fmrole M) (_ : nat),
-          if decide (ρ' ∈ dom (ls_fuel δ1)) then ls_mapping δ1 !! ρ' else Some ζ)
-       (gset_to_gmap 333 ((dom (ls_fuel δ1) ∪ dom fs2) ∖ (dom fs1 ∖ dom fs2))))
-    (<[ζ:=dom fs2]> (ls_tmap δ1 (LM := LM))).
-Proof. 
-  intros ρ' ζ'. simpl. rewrite map_lookup_imap.
-  rewrite lookup_gset_to_gmap //=.
-  destruct (decide (ρ' ∈ (dom (ls_fuel δ1) ∪ dom fs2) ∖ (dom fs1 ∖ dom fs2))) as [Hin|Hnotin].
-  - rewrite option_guard_True //=. destruct (decide (ρ' ∈ dom (ls_fuel δ1))).
-    + destruct (decide (ζ' = ζ)) as [->|Hneq].
-      * rewrite lookup_insert. split.
-        { eexists; split =>//. apply elem_of_difference in Hin as [? Hin].
-          apply not_elem_of_difference in Hin as [?|?]; [|done].
-          rewrite decide_True in H; [set_solver| ]. done. }
-        { intros (?&?&?). simplify_eq.
-          rewrite decide_True; [| set_solver]. 
-          apply Hxdom.
-          destruct Hfuelsval as (?&?&?&?&?). by_contradiction.
-          assert (ρ' ∈ live_roles M s2 ∖ live_roles M δ1).
-          { set_solver. }
-          assert (ρ' ∈ fr1).
-          { set_solver. }
-          assert (ρ' ∉ dom $ ls_fuel δ1) by set_solver.
-          done. }
-      * rewrite lookup_insert_ne //. rewrite decide_True; [| done]. 
-        apply ls_mapping_tmap_corr.
-    + split.
-      * rewrite decide_False; [| done]. 
-        intros Htid. simplify_eq.
-        rewrite lookup_insert. eexists; split=>//.
-        set_solver.
-      * rewrite decide_False; [| done]. 
-        assert (ρ' ∈ dom fs2) by set_solver. intros Hm. by_contradiction.
-        rewrite lookup_insert_ne in Hm; last congruence.
-        apply ls_mapping_tmap_corr in Hm.
-        apply elem_of_dom_2 in Hm. rewrite ls_same_doms // in Hm.
-  - destruct Hfuelsval as (?&?&?&?&Hinf&?). rewrite option_guard_False //=. split; first done.
-    destruct (decide (ζ' = ζ)) as [->|Hneq].
-    { rewrite lookup_insert //. intros (?&?&?). simplify_eq. set_solver. }
-    rewrite lookup_insert_ne //.
-    intros Habs%ls_mapping_tmap_corr.
-    
-    apply not_elem_of_difference in Hnotin as [Hnin|Hin].
-    + apply elem_of_dom_2 in Habs. rewrite ls_same_doms in Habs. set_solver.
-    + apply elem_of_difference in Hin as [Hin Hnin].
-      apply Hxdom in Hin. rewrite Hin in Habs. congruence.  
-Qed.       
