fairness/heap_lang/em_lm_heap_lang.v
@@ -1,0 +1,274 @@
+From trillium.fairness.heap_lang Require Import heap_lang_defs em_lm.
+
+
+Section LM_EM_HL.
+  Context `{LM: LiveModel (locale heap_lang) M}. 
+
+  Definition LM_EM_HL: ExecutionModel heap_lang LM :=
+    LM_EM (LM := LM) 0%nat ltac:(done).
+
+  Global Instance LM_EM_fairPre `{hGS: @heapGpreS Σ LM LM_EM_HL}:
+    fairnessGpreS LM Σ.
+  Proof. apply hGS. Defined. 
+
+(* TODO: get rid of it*)
+  Global Instance LM_EM_fair `{hGS: @heapGS Σ LM LM_EM_HL}:
+    fairnessGS LM Σ.
+  Proof. apply hGS. Defined.
+
+End LM_EM_HL.
+
+Lemma tids_smaller_restrict_mapping `{M: FairModel}
+  (c1 c2: cfg heap_lang) δ1 δ2 (ζ: locale heap_lang)
+  (Hζs : tids_smaller c1.1 δ1)
+  (DOM12: ls_mapping δ2 ⊆ ls_mapping δ1)
+  (STEP: locale_step c1 (Some ζ) c2)
+  :
+  tids_smaller c2.1 δ2 (M := M).
+Proof.
+  unfold tids_smaller; simpl.
+  intros ρ ζ0 Hin.
+  destruct c1, c2.
+  eapply from_locale_step =>//.
+  rewrite /tids_smaller /= in Hζs. eapply Hζs.
+  eapply lookup_weaken; eauto. 
+Qed.
+
+Lemma tids_dom_restrict_mapping `{LM: LiveModel (locale heap_lang) M} 
+  (c1 c2: cfg heap_lang)
+  (tmap1 tmap2: gmap (locale heap_lang) (gset (fmrole M))) (ζ: locale heap_lang)
+  (Hstep : locale_step c1 (Some ζ) c2)
+  (Hlocssmall: tids_restrict c1 tmap1)
+  (TMAP2: exists S, tmap2 = <[ζ:=S]> (tmap1))
+  :
+  tids_restrict c2 tmap2.
+Proof.
+  intros ζ0 Hnotin.
+  destruct TMAP2 as [? ->]. 
+  destruct c1, c2. simpl in *. 
+  apply lookup_insert_None; split.
+  + apply Hlocssmall.
+    have Hle := locales_of_list_step_incl _ _ _ _ _ Hstep. simpl.
+    clear -Hnotin Hle. set_solver.
+  + intros <-. 
+    have ? := locales_of_list_step_incl _ _ _ _ _ Hstep. simpl.
+    (* clear Hfueldom Hsamedoms. *)
+    inversion Hstep. simplify_eq.
+    assert (locale_of t1 e1 ∈ locales_of_list (t1 ++ e1 :: t2));
+      last by eauto.
+    apply locales_of_list_from_locale_from.
+    rewrite from_locale_from_Some //. 
+    eapply prefixes_from_spec.
+    eexists _,_. by list_simplifier.
+Qed.
+  (* TODO: ?? *)
+    (* - rewrite Hnewdom /new_dom. apply elem_of_equiv_empty_L. intros ρ [Hin1 Hin2]%elem_of_intersection. *)
+    (*   assert (ρ ∈ dom (ls_fuel δ1)) *)
+    (*     by set_solver -Hnewdom Hsamedoms Hfueldom. *)
+    (*   set_solver -Hnewdom Hsamedoms Hfueldom. } *) 
+
+
+Lemma tids_smaller_fork_step `{LM: LiveModel (locale heap_lang) M}  σ1 σ2 δ1 δ2 ζ τ_new
+  (Hstep: locale_step σ1 (Some ζ) σ2)
+  (SM: tids_smaller σ1.1 δ1)
+  (MAP2: exists (R2: gset (fmrole M)), ls_mapping δ2 = map_imap
+                                                    (λ (ρ : fmrole M) (o : locale heap_lang),
+                                                      if decide (ρ ∈ R2) then Some τ_new else Some o)
+                                                    (ls_mapping δ1))
+  (FORK: ∃ tp1' efork, τ_new = locale_of σ1.1 efork /\ σ2.1 = tp1' ++ [efork] ∧ length tp1' = length σ1.1)
+  :
+  tids_smaller σ2.1 δ2 (M := M).
+Proof.
+  destruct σ1 as [tp1 σ1], σ2 as [tp2 σ2]. simpl in *.
+  intros ρ ζ'.
+  simpl in *. destruct MAP2 as [R2 ->].
+  simpl. rewrite map_lookup_imap.
+  destruct (ls_mapping δ1 !!ρ) eqn:Heq.
+  2: { intros. simpl in *. discriminate. }
+  
+  destruct (decide (ρ ∈ R2)); first  (intros ?; simplify_eq).
+  - destruct FORK as (tp1' & efork & (-> & -> & Hlen)).
+    inversion Hstep as [? ? e1 ? e2 ? efs t1 t2 Hf1 YY Hprimstep |]. simplify_eq.
+    assert (efs = [efork]) as ->.
+    { symmetry. assert (length tp1' = length (t1 ++ e2 :: t2)).
+      rewrite app_length //=; rewrite app_length //= in Hlen.
+      clear Hlen. eapply app_inj_1 =>//. by list_simplifier. }
+    inversion H.
+    subst ζ'. 
+    assert (is_Some (from_locale (t1 ++ e1 :: t2 ++ [efork]) (locale_of (t1 ++ e1 :: t2) efork))).
+    + unfold from_locale. erewrite from_locale_from_Some; eauto.
+      apply prefixes_from_spec. list_simplifier. eexists _, []. split=>//.
+      by list_simplifier.
+    + eapply from_locale_from_equiv =>//; [constructor |].
+      (* rewrite H0. *)
+      replace (t1 ++ e1 :: t2 ++ [efork]) with ((t1 ++ e1 :: t2) ++ [efork]);
+        last by list_simplifier.
+      replace (t1 ++ e2 :: t2 ++ [efork]) with ((t1 ++ e2 :: t2) ++ [efork]);
+        last by list_simplifier.
+      assert (locales_equiv (t1 ++ e1 :: t2) (t1 ++ e2 :: t2)).
+      { apply locales_equiv_middle. eapply locale_step_preserve =>//. }
+      assert (tp1' = t1 ++ e2 :: t2).
+      { rewrite app_comm_cons in YY. 
+        erewrite app_assoc in YY. eapply app_inj_tail in YY. apply YY. }
+      apply locales_equiv_from_app =>//.
+      * congruence.
+      * eapply locales_equiv_from_refl. by list_simplifier. 
+  - intros ?; simplify_eq.
+    assert (is_Some (from_locale tp1 ζ')). 
+    2: by eapply from_locale_step =>//.
+    inversion H. subst. eauto. 
+Qed.
+
+Lemma tids_dom_fork_step `{LM: LiveModel (locale heap_lang) M}
+  (c1 c2: cfg heap_lang) (ζ: locale heap_lang)
+  (tmap1 tmap2: gmap (locale heap_lang) (gset (fmrole M)))
+  τ_new (R1 R2: gset (fmrole M))
+  (Hstep: locale_step c1 (Some ζ) c2)
+  (Hsmall: ∀ ζ : locale heap_lang,
+      ζ ∉ locales_of_list c1.1 → tmap1 !! ζ = None)
+  (Hmapping : ζ ∈ dom tmap1)
+  (FORK: (∃ tp1' efork, τ_new = locale_of c1.1 efork /\ c2.1 = tp1' ++ [efork] ∧ length tp1' = length c1.1))
+  (TMAP2: tmap2 = <[τ_new:=R2]> (<[ζ:=R1]> (tmap1)))
+  :
+  ∀ ζ0 : locale heap_lang,
+    ζ0 ∉ locales_of_list c2.1 → tmap2 !! ζ0 = None.
+Proof.
+  assert (Hlocincl: locales_of_list c1.1 ⊆ locales_of_list c2.1).
+  { destruct c1 as [tp1 σ1], c2 as [tp2 σ2]. simpl in *.
+    apply (locales_of_list_step_incl _ _ _ _ _ Hstep). }
+  intros ζ' Hζ'.
+  rewrite TMAP2.
+  destruct c1 as [tp1 σ1], c2 as [tp2 σ2]. simpl in *.
+  rewrite lookup_insert_ne.
+  { rewrite lookup_insert_ne; last first.
+    { intros <-.
+      apply elem_of_dom in Hmapping as [? MM]. 
+      rewrite Hsmall in MM; [congruence | naive_solver]. }
+    apply Hsmall; set_unfold; naive_solver. }
+  pose proof (locales_of_list_step_incl _ _ _ _ _ Hstep).
+  (* clear Hfueldom Hsamedoms. *)
+  assert (ζ' ∉ locales_of_list tp1) by eauto.
+  intros contra. simplify_eq.
+  destruct FORK as (tp1' & efork & (-> & -> & Hlen)).
+  inversion Hstep as [? ? e1 ? e2 ? efs t1 t2 Hf1 YY Hprimstep |].
+  simplify_eq.
+  assert (efs = [efork]) as ->.
+  { symmetry. assert (length tp1' = length (t1 ++ e2 :: t2)).
+    rewrite app_length //=; rewrite app_length //= in Hlen.
+    clear Hlen. eapply app_inj_1 =>//. by list_simplifier. }
+  (* rewrite H0 in Hζ'. *)
+  apply Hζ'. apply elem_of_list_fmap.
+  eexists (t1 ++ e2 :: t2, _); split =>//.
+  - erewrite locale_equiv =>//. apply locales_equiv_middle.
+    eapply locale_step_preserve => //.
+  - replace (t1 ++ e2 :: t2 ++ [efork]) with ((t1 ++ e2 :: t2) ++ [efork]); last by list_simplifier.
+    rewrite prefixes_from_app.
+    rewrite app_comm_cons app_assoc in YY. eapply app_inj_tail in YY.
+    set_unfold; naive_solver.
+Qed.
+
+
+Lemma tids_smaller_model_step `{LM: LiveModel (locale heap_lang) M} c1 c2 ζ δ1 δ2
+  (Hstep: locale_step c1 (Some ζ) c2)
+  (Hless: tids_smaller c1.1 δ1)
+  (* S is a subset of dom (ls_fuel δ1); *)
+  (*      missing roles are those that are dropped by ζ; *)
+  (*      new roles get assigned here *)
+  (MAP2: exists f (S: gset (fmrole M)),
+      ls_mapping δ2 = map_imap
+                        (λ (ρ' : fmrole M) (_ : nat),
+                          if decide (ρ' ∈ dom (ls_fuel δ1))
+                          then ls_mapping δ1 !! ρ'
+                          else Some ζ)
+                        (gset_to_gmap f S)
+  )
+  :
+  tids_smaller c2.1 δ2 (M := M).
+Proof.  
+  (* eapply tids_smaller_restrict_mapping; eauto. *)
+  (* destruct MAP2 as (?&?&->).   *)
+  unfold tids_smaller; simpl.
+  simpl in MAP2. destruct MAP2 as (?&S&->).
+  intros ρ' ? Hmim.
+  rewrite map_lookup_imap in Hmim. rewrite lookup_gset_to_gmap in Hmim.
+  destruct (decide (ρ' ∈ S)); last by rewrite option_guard_False in Hmim.
+  rewrite option_guard_True //= in Hmim.
+  destruct (decide (ρ' ∈ dom (ls_fuel δ1))). 
+  + inversion Hstep; simplify_eq.
+    eapply from_locale_step =>//. eapply Hless. rewrite -Hmim decide_True; auto. 
+  + simplify_eq.
+    inversion Hstep; simplify_eq.
+    eapply from_locale_step =>//. unfold from_locale.
+    simpl. rewrite decide_False in Hmim; [| done]. inversion Hmim. subst ζ0.  
+    rewrite from_locale_from_Some; [done| ]. 
+    apply prefixes_from_spec. exists t1, t2. by list_simplifier.
+Qed.
+
+Ltac by_contradiction :=
+  match goal with
+  | |- ?goal => destruct_decide (decide (goal)); first done; exfalso
+  end.
+
+Lemma mim_helper_model_step `{LM: LiveModel (locale heap_lang) M}
+  (s2 : fmstate M)
+  (fs1 fs2 : gmap (fmrole M) nat)
+  (ρ : fmrole M)
+  (δ1 : LM)
+  (ζ : locale heap_lang)
+  (fr1 : gset (fmrole M))
+  (Hfr_new : live_roles M s2 ∖ live_roles M δ1 ⊆ fr1)
+  (Hfuelsval : valid_new_fuelmap fs1 fs2 δ1 s2 ρ (LM := LM))
+  (Hxdom : ∀ ρ : fmrole M, ls_mapping δ1 !! ρ = Some ζ ↔ ρ ∈ dom fs1)
+  (HFR : fr1 ∩ dom (ls_fuel δ1) = (∅: gset (fmrole M))):
+  maps_inverse_match
+    (map_imap
+       (λ (ρ' : fmrole M) (_ : nat),
+          if decide (ρ' ∈ dom (ls_fuel δ1)) then ls_mapping δ1 !! ρ' else Some ζ)
+       ((gset_to_gmap 333%nat ((dom (ls_fuel δ1) ∪ dom fs2) ∖ (dom fs1 ∖ dom fs2)))
+         (* : gmap (fmrole M) (locale heap_lang) *)
+)
+)
+    (<[ζ:=dom fs2]> (ls_tmap δ1 (LM := LM))).
+Proof. 
+  intros ρ' ζ'. simpl. rewrite map_lookup_imap.
+  rewrite lookup_gset_to_gmap //=.
+  destruct (decide (ρ' ∈ (dom (ls_fuel δ1) ∪ dom fs2) ∖ (dom fs1 ∖ dom fs2))) as [Hin|Hnotin].
+  - rewrite option_guard_True //=. destruct (decide (ρ' ∈ dom (ls_fuel δ1))).
+    + destruct (decide (ζ' = ζ)) as [->|Hneq].
+      * rewrite lookup_insert. split.
+        { eexists; split =>//. apply elem_of_difference in Hin as [? Hin].
+          apply not_elem_of_difference in Hin as [?|?]; [|done].
+          rewrite decide_True in H; [set_solver| ]. done. }
+        { intros (?&?&?). simplify_eq.
+          rewrite decide_True; [| set_solver]. 
+          apply Hxdom.
+          destruct Hfuelsval as (?&?&?&?&?). by_contradiction.
+          assert (ρ' ∈ live_roles M s2 ∖ live_roles M δ1).
+          { set_solver. }
+          assert (ρ' ∈ fr1).
+          { set_solver. }
+          assert (ρ' ∉ dom $ ls_fuel δ1) by set_solver.
+          done. }
+      * rewrite lookup_insert_ne //. rewrite decide_True; [| done]. 
+        apply ls_mapping_tmap_corr.
+    + split.
+      * rewrite decide_False; [| done]. 
+        intros Htid. simplify_eq.
+        rewrite lookup_insert. eexists; split=>//.
+        set_solver.
+      * rewrite decide_False; [| done]. 
+        assert (ρ' ∈ dom fs2) by set_solver. intros Hm. by_contradiction.
+        rewrite lookup_insert_ne in Hm; last congruence.
+        apply ls_mapping_tmap_corr in Hm.
+        apply elem_of_dom_2 in Hm. rewrite ls_same_doms // in Hm.
+  - destruct Hfuelsval as (?&?&?&?&Hinf&?). rewrite option_guard_False //=. split; first done.
+    destruct (decide (ζ' = ζ)) as [->|Hneq].
+    { rewrite lookup_insert //. intros (?&?&?). simplify_eq. set_solver. }
+    rewrite lookup_insert_ne //.
+    intros Habs%ls_mapping_tmap_corr.
+    
+    apply not_elem_of_difference in Hnotin as [Hnin|Hin].
+    + apply elem_of_dom_2 in Habs. rewrite ls_same_doms in Habs. set_solver.
+    + apply elem_of_difference in Hin as [Hin Hnin].
+      apply Hxdom in Hin. rewrite Hin in Habs. congruence.  
+Qed.       
